examples/nsl_pk/DY.Example.NSL.Protocol.Total.Proof.fst
@@ -23,8 +23,7 @@ let crypto_predicates_nsl = {
 
   pkenc_pred = {
     pred = (fun tr pk msg ->
-      get_sk_usage pk == PkKey "NSL.PublicKey" empty /\
-      (exists prin. get_sk_label pk = principal_label prin /\ (
+      (exists prin. get_sk_usage pk == PkKey "NSL.PublicKey" (serialize private_key_principal prin) /\ (
         match parse message msg with
         | Some (Msg1 msg1) -> (
           let (alice, bob) = (msg1.alice, prin) in
@@ -71,17 +70,13 @@ val compute_message1_proof:
     // From random generation
     PkNonce? (get_usage nonce) /\
     // From PKI invariants
-    is_encryption_key (PkKey "NSL.PublicKey" empty) (principal_label bob) tr pk_b
+    is_encryption_key (PkKey "NSL.PublicKey" (serialize private_key_principal bob)) (principal_label bob) tr pk_b
   )
   (ensures is_publishable tr (compute_message1 alice bob pk_b n_a nonce))
 let compute_message1_proof tr alice bob pk_b n_a nonce =
   let msg = Msg1 {n_a; alice;} in
   serialize_wf_lemma message (is_knowable_by (principal_label alice) tr) msg;
-  serialize_wf_lemma message (is_knowable_by (principal_label bob) tr) msg;
-  
-  let pk = pk_b in
-  let msg = (serialize message msg) in
-  assume(pkenc_pred.pred tr pk msg)
+  serialize_wf_lemma message (is_knowable_by (principal_label bob) tr) msg
 
 // If bob successfully decrypt the first message,
 // then n_a is knownable both by alice (in the message) and bob (the principal)
@@ -95,7 +90,7 @@ val decode_message1_proof:
   Lemma
   (requires
     // From PrivateKeys invariants
-    is_decryption_key (PkKey "NSL.PublicKey" empty) (principal_label bob) tr sk_b /\
+    is_decryption_key (PkKey "NSL.PublicKey" (serialize private_key_principal bob)) (principal_label bob) tr sk_b /\
     // From the network
     bytes_invariant tr msg_cipher
   )
@@ -131,7 +126,7 @@ val compute_message2_proof:
     // From the random generation
     PkNonce? (get_usage nonce) /\
     // From the PKI
-    is_encryption_key (PkKey "NSL.PublicKey" empty) (principal_label msg1.alice) tr pk_a
+    is_encryption_key (PkKey "NSL.PublicKey" (serialize private_key_principal msg1.alice)) (principal_label msg1.alice) tr pk_a
   )
   (ensures
     is_publishable tr (compute_message2 bob msg1 pk_a n_b nonce)
@@ -139,8 +134,7 @@ val compute_message2_proof:
 let compute_message2_proof tr bob msg1 pk_a n_b nonce =
   let msg = Msg2 {n_a = msg1.n_a;  n_b; bob;} in
   serialize_wf_lemma message (is_knowable_by (principal_label msg1.alice) tr) msg;
-  serialize_wf_lemma message (is_knowable_by (principal_label bob) tr) msg;
-  admit()
+  serialize_wf_lemma message (is_knowable_by (principal_label bob) tr) msg
 
 // If alice successfully decrypt the second message,
 // then n_b is knownable both by alice (in the message) and bob (the principal)
@@ -156,7 +150,7 @@ val decode_message2_proof:
     // From the NSL state invariant
     is_secret (join (principal_label alice) (principal_label bob)) tr n_a /\
     // From the PrivateKeys invariant
-    is_decryption_key (PkKey "NSL.PublicKey" empty) (principal_label alice) tr sk_a /\
+    is_decryption_key (PkKey "NSL.PublicKey" (serialize private_key_principal alice)) (principal_label alice) tr sk_a /\
     // From the network
     bytes_invariant tr msg_cipher
   )
@@ -178,7 +172,8 @@ let decode_message2_proof tr alice bob msg_cipher sk_a n_a =
     let Some msg = pk_dec sk_a msg_cipher in
     FStar.Classical.move_requires (parse_wf_lemma message (is_publishable tr)) msg;
     FStar.Classical.move_requires (parse_wf_lemma message (bytes_invariant tr)) msg;
-    admit()
+    //TODO why do we need this assert?
+    assert(is_publishable tr n_a ==> (join (principal_label alice) (principal_label bob)) `can_flow tr` public)
   )
 #pop-options
 
@@ -196,7 +191,7 @@ val compute_message3_proof:
     // From the random generation
     PkNonce? (get_usage nonce) /\
     // From the PKI
-    is_encryption_key (PkKey "NSL.PublicKey" empty) (principal_label bob) tr pk_b
+    is_encryption_key (PkKey "NSL.PublicKey" (serialize private_key_principal bob)) (principal_label bob) tr pk_b
   )
   (ensures
     is_publishable tr (compute_message3 alice bob pk_b n_b nonce)
@@ -207,8 +202,7 @@ let compute_message3_proof tr alice bob pk_b n_b nonce =
   serialize_wf_lemma message (is_knowable_by (principal_label alice) tr) msg;
   serialize_wf_lemma message (is_knowable_by (principal_label bob) tr) msg;
   let msg3: message3 = {n_b;} in
-  assert(msg3.n_b == n_b);
-  admit()
+  assert(msg3.n_b == n_b)
 
 // If bob successfully decrypt the third message,
 // Then either alice or bob are corrupt, or alice triggered the Initiate2 event
@@ -222,7 +216,7 @@ val decode_message3_proof:
     // From the NSL state invariant
     get_label n_b `equivalent tr` join (principal_label alice) (principal_label bob) /\
     // From the PrivateKeys invariant
-    is_decryption_key (PkKey "NSL.PublicKey" empty) (principal_label bob) tr sk_b /\
+    is_decryption_key (PkKey "NSL.PublicKey" (serialize private_key_principal bob)) (principal_label bob) tr sk_b /\
     // From the network
     bytes_invariant tr msg_cipher
   )
@@ -244,6 +238,7 @@ let decode_message3_proof tr alice bob msg_cipher sk_b n_b =
     let Some msg = pk_dec sk_b msg_cipher in
     FStar.Classical.move_requires (parse_wf_lemma message (is_publishable tr)) msg;
     FStar.Classical.move_requires (parse_wf_lemma message (bytes_invariant tr)) msg;
-    admit()
+    //TODO why do we need this assert?
+    assert(is_publishable tr n_b ==> (join (principal_label alice) (principal_label bob)) `can_flow tr` public)
   )
 #pop-options
