examples/iso_dh/DY.Example.DH.Protocol.Total.Proof.fst
@@ -37,8 +37,8 @@ let dh_crypto_preds = {
 
   sign_pred = {
     pred = (fun tr vk sig_msg ->
-      get_signkey_usage vk == SigKey "DH.SigningKey" empty /\
-      (exists prin. get_signkey_label vk = principal_label prin /\ (
+      
+      (exists prin. get_signkey_usage vk == SigKey "DH.SigningKey" (serialize private_key_principal prin) /\ (
         match parse sig_message sig_msg with
         | Some (SigMsg2 sig_msg2) -> (
           exists y. sig_msg2.gy == (dh_pk y) /\ event_triggered tr prin (Respond1 sig_msg2.alice prin sig_msg2.gx sig_msg2.gy y)
@@ -130,7 +130,7 @@ val compute_message2_proof:
     event_triggered tr bob (Respond1 alice bob gx (dh_pk y) y) /\
     is_publishable tr gx /\
     bytes_invariant tr y /\
-    is_signature_key (SigKey "DH.SigningKey" empty) (principal_label bob) tr sk_b /\
+    is_signature_key (SigKey "DH.SigningKey" (serialize private_key_principal bob)) (principal_label bob) tr sk_b /\
     is_secret (principal_label bob) tr n_sig /\
     SigNonce? (get_usage n_sig)
   )
@@ -175,7 +175,7 @@ val decode_and_verify_message2_proof:
   (requires
     is_publishable tr msg2_bytes /\
     is_secret (principal_state_label alice alice_si) tr x /\
-    is_verification_key (SigKey "DH.SigningKey" empty) (principal_label bob) tr pk_b
+    is_verification_key (SigKey "DH.SigningKey" (serialize private_key_principal bob)) (principal_label bob) tr pk_b
   )
   (ensures (
     match decode_and_verify_message2 msg2_bytes alice x pk_b with
@@ -218,7 +218,7 @@ val compute_message3_proof:
     event_triggered tr alice (Initiate2 alice bob (dh_pk x) gy (dh x gy)) /\
     is_publishable tr gx /\ is_publishable tr gy /\
     gx = dh_pk x /\
-    is_signature_key (SigKey "DH.SigningKey" empty) (principal_label alice) tr sk_a /\
+    is_signature_key (SigKey "DH.SigningKey" (serialize private_key_principal alice)) (principal_label alice) tr sk_a /\
     is_secret (principal_label alice) tr n_sig /\
     SigNonce? (get_usage n_sig)
   )
@@ -259,7 +259,7 @@ val decode_and_verify_message3_proof:
     is_publishable tr msg3_bytes /\
     is_publishable tr gx /\
     is_secret (principal_state_label bob bob_si) tr y /\
-    is_verification_key (SigKey "DH.SigningKey" empty) (principal_label alice) tr pk_a
+    is_verification_key (SigKey "DH.SigningKey" (serialize private_key_principal alice)) (principal_label alice) tr pk_a
   )
   (ensures (
     let gy = dh_pk y in
